\documentclass[a4paper]{article}
% Русский язык
\usepackage[utf8]{inputenc}
\usepackage[russian]{babel}
% Математические символы и формулы
\usepackage{mathtools}
\usepackage{float}
% Разбиение на разные файлы
\usepackage{subfiles}
% Отступы с краев(margin)
\usepackage[margin=1in]{geometry}
% Форматирование заголовков
\usepackage{titlesec}
\usepackage{indentfirst} % Красная строка
% Схемки
% \usepackage{circuitikz}
% Картинки
\usepackage{graphicx}
\usepackage{breqn}

\begin{document}

\section{INPUT}
$A_r$, $A_ii$, $B_r$, $B_i$

\section{FORMULA}
$$ y_r + y_ii = (A_r + A_ii)(x_r + x_ii) + B_r + B_ii $$

\section{YR}
$$ y_r = (A_r + A_ii)(x_r + x_ii) + B_r + B_ii - y_ii$$

\section{YI}
$$ y_i = \frac{(A_r + A_ii)(x_r + x_ii) + B_r + B_ii - y_r}{i} $$

\section{XR}
$$ x_r = \frac{y_r + y_ii - (A_r + A_ii)(x_ii) - B_r - B_ii}{A_r + A_ii} $$

\section{XI}
$$ x_i = \frac{y_r + y_ii - (A_r + A_ii)(x_r) - B_r - B_ii}{A_r + A_ii} $$

\section{abc}
$$ y_r = (A_r + A_ii)(x_r + x_ii) + B_r + B_ii - y_ii $$

\subsection{$x_r = 0, x_i = 0, y_i = 0$}
$$ y_r = (A_r + A_ii)(0 + 0) + B_r + B_ii - 0i = B_r + B_ii = B_r $$

\subsection{$x_r = 1, x_i = 0, y_i = 0$}
$$ y_r = (A_r + A_ii)(1 + 0i) + B_r + B_ii - 0i = A_r + A_ii + B_r + B_ii = A_r + B_r $$

\subsection{$x_r = 0, x_i = 1, y_i = 0$}
$$ y_r = (A_r + A_ii)(0 + i) + B_r + B_ii - 0i = A_ri - A_i + B_r + B_ii = B_r - A_i $$

\section{abc2}
\subsection{$x_r = 0, x_i = 0, y_r = 0$}
$$ y_i = -B_r + B_i $$

\subsection{$x_r = 1, x_i = 0, y_r = 0$}
$$ y_i = -A_r + A_i - B_r + B_i $$

\subsection{$x_r = 0, x_i = 1, y_r = 0$}
$$ y_i = A_r + A_i - B_r + B_i $$


\subsubsection{$ Ax + By + Cz + D = 0 $}
\begin{table}[h]
    \centering
    \begin{tabular}{| c c c |}
        $x - x_0 $ & $ x_1 - x_0 $ & $ x_2 - x_0 $ \\
        $y - y_0 $ & $ y_1 - y_0 $ & $ x_2 - x_0 $ \\
        $z - z_0 $ & $ z_1 - x_0 $ & $ x_2 - x_0 $ \\
    \end{tabular}
\end{table}

$$ x = x_r $$
$$ y = y_r $$
$$ z = x_i $$
\begin{table}[h]
    \centering
    \begin{tabular}{| c c c |}
        $x - 0$   & $ 1 - 0           $ & $ 0 - 0$ \\
        $y - B_r$ & $ A_r + B_r - B_r $ & $ -A_i + B_r - B_r $ \\
        $z - 0$   & $ 0 - 0           $ & $ 1 - 0$ \\
    \end{tabular}
\end{table}


\section{OUTPUT}
$A_1$, $B_1$, $C_1$, $D_1$,
$A_2$, $B_2$, $C_2$, $D_2$,


\end{document}
